feat(*) prepare afp submission

Transport/Examples/Prototype/Transport_Prototype.thy
@@ -88,61 +88,36 @@ qed
 
 end
 
+lemmas related_Fun_Rel_combI = Dep_Fun_Rel_relD[where ?S="\<lambda>_ _. S" for S, rotated]
+lemma related_Fun_Rel_lambdaI:
+  assumes "\<And>x y. R x y \<Longrightarrow> S (f x) (g y)"
+  and "T = (R \<Rrightarrow> S)"
+  shows "T f g"
+  using assms by blast
+
+
 paragraph \<open>General ML setups\<close>
-
 ML_file\<open>transport_util.ML\<close>
-
-ML\<open>
-  structure Util = Transport_Util
-  val transport_id = "trp"
-\<close>
-
-paragraph \<open>Simplifying Definitions\<close>
-
-ML\<open>
-  val simp_rhs = Simplifier.rewrite #> Conversion_Util.rhs_conv #> Conversion_Util.thm_conv
-
-  \<comment> \<open>simplifies the generated definition of a transported term\<close>
-  fun simp_transported_def ctxt simps y_def =
-    let
-      val ctxt = ctxt addsimps simps
-      val y_def_eta_expanded = Util.equality_eta_expand ctxt "x" y_def
-    in apply2 (simp_rhs ctxt) (y_def, y_def_eta_expanded) end
-\<close>
-
-text \<open>Definitions used by Transport that need to be folded before a PER proof and unfolded after
-success.\<close>
-ML\<open>
-  structure Transport_Defs = Named_Thms(
-    val name = @{binding "transport_def"}
-    val description = "Definitions used by Transport"
-  )
-  val _ = Theory.setup Transport_Defs.setup
-\<close>
-
-declare
-  transport_Dep_Fun_Rel.transport_defs[transport_def]
-  transport_Fun_Rel.transport_defs[transport_def]
 
 paragraph \<open>Unification Setup\<close>
 
 ML\<open>
   @{functor_instance struct_name = Transport_Unification_Combine
     and functor_name = Unification_Combine
-    and id = transport_id}
+    and id = Transport_Util.transport_id}
 \<close>
 local_setup \<open>Transport_Unification_Combine.setup_attribute NONE\<close>
 ML\<open>
   @{functor_instance struct_name = Transport_Mixed_Unification
     and functor_name = Mixed_Unification
-    and id = transport_id
+    and id = Transport_Util.transport_id
     and more_args = \<open>structure UC = Transport_Unification_Combine\<close>}
 \<close>
 
 ML\<open>
   @{functor_instance struct_name = Transport_Unification_Hints
     and functor_name = Term_Index_Unification_Hints
-    and id = transport_id
+    and id = Transport_Util.transport_id
     and more_args = \<open>
       structure TI = Discrimination_Tree
       val init_args = {
@@ -165,33 +140,12 @@ declare [[trp_ucombine add = \<open>Transport_Unification_Combine.eunif_data
   |> K)
   (Transport_Unification_Combine.default_metadata Transport_Unification_Hints.binding)\<close>]]
 
-paragraph \<open>Resolution Setup\<close>
+paragraph \<open>Prototype\<close>
+ML_file\<open>transport.ML\<close>
 
-ML\<open>
-  \<comment> \<open>resolution with above unifier\<close>
-  val any_unify_trp_hints_resolve_tac = Unify_Resolve_Base.unify_resolve_any_tac
-    Transport_Mixed_Unification.norms_first_higherp_first_comb_higher_unify
-    Transport_Mixed_Unification.first_higherp_first_comb_higher_unify
-
-  fun get_theorems_tac f get_theorems ctxt = f (get_theorems ctxt) ctxt
-  val get_theorems_resolve_tac = get_theorems_tac any_unify_trp_hints_resolve_tac
-\<close>
-
-method_setup trp_hints_resolve =
-  \<open>Attrib.thms >> (SIMPLE_METHOD' oo any_unify_trp_hints_resolve_tac)\<close>
-  "Resolution with unification hints for Transport "
-
-paragraph \<open>PER equivalence prover\<close>
-
-text \<open>Introduction rules.\<close>
-
-ML\<open>
-  structure PER_Intros = Named_Thms(
-    val name = @{binding "per_intro"}
-    val description = "Introduction rules for per_prover"
-  )
-  val _ = Theory.setup PER_Intros.setup
-\<close>
+declare
+  transport_Dep_Fun_Rel.transport_defs[trp_def]
+  transport_Fun_Rel.transport_defs[trp_def]
 
 declare
   (*dependent case currently disabled by default since they easily make the
@@ -206,381 +160,9 @@ declare
   transport_eq_id.partial_equivalence_rel_equivalenceI[per_intro]
   transport_eq_restrict_id.partial_equivalence_rel_equivalence[per_intro]
 
-ML\<open>
-  fun per_prover_tac ctxt = REPEAT_ALL_NEW (get_theorems_resolve_tac PER_Intros.get ctxt)
-\<close>
-
-method_setup per_prover =
-  \<open>Scan.succeed (SIMPLE_METHOD' o per_prover_tac)\<close>
-  "PER prover for Transport"
-
-
-paragraph \<open>Domain Prover\<close>
-
-ML\<open>
-  structure Transport_in_dom = Named_Thms(
-    val name = @{binding "transport_in_dom"}
-    val description = "In domain theorems for Transport"
-  )
-  val _ = Theory.setup Transport_in_dom.setup
-\<close>
-
-text \<open>Discharges the @{term "L x x'"} goals by registered lemmas.\<close>
-ML\<open>
-  fun transport_in_dom_prover_tac ctxt = get_theorems_resolve_tac Transport_in_dom.get ctxt
-\<close>
-
-method_setup transport_in_dom_prover =
-  \<open>Scan.succeed (SIMPLE_METHOD' o transport_in_dom_prover_tac)\<close>
-  "in_dom prover for Transport"
-
-
-paragraph \<open>Blackbox Prover\<close>
-
-text \<open>First derives the PER equivalence, then looks for registered domain lemmas.\<close>
-ML\<open>
-  fun unfold_tac thms ctxt = simp_tac (clear_simpset ctxt addsimps thms)
-  val unfold_transport_defs_tac = get_theorems_tac unfold_tac Transport_Defs.get
-
-  fun transport_prover ctxt i =
-    per_prover_tac ctxt i
-    THEN TRY (SOMEGOAL
-      (TRY o unfold_transport_defs_tac ctxt
-      THEN' transport_in_dom_prover_tac ctxt)
-    )
-\<close>
-
-method_setup transport_prover =
-  \<open>Scan.succeed (SIMPLE_METHOD' o transport_prover)\<close>
-  "Blackbox prover for Transport"
-
-
-paragraph \<open>Whitebox Prover Intro Rules\<close>
-
-ML\<open>
-  structure Transport_Related_Intros = Named_Thms(
-    val name = @{binding "transport_related_intro"}
-    val description = "Introduction rules for Transport whitebox proofs"
-  )
-  val _ = Theory.setup Transport_Related_Intros.setup
-\<close>
-
-
-paragraph \<open>Relator Rewriter\<close>
-
-text \<open>Rewrite rules to simplify the derived Galois relator.\<close>
-ML\<open>
-  structure Transport_Relator_Rewrites = Named_Thms(
-    val name = @{binding "transport_relator_rewrite"}
-    val description = "Rewrite rules for relators used by Transport"
-  )
-  val _ = Theory.setup Transport_Relator_Rewrites.setup
-\<close>
-
 declare
-  transport_id.left_Galois_eq_left[transport_relator_rewrite]
-  transport_Fun_Rel.left_Galois_eq_Fun_Rel_left_Galois[transport_relator_rewrite]
-
-ML\<open>
-  (*simple rewrite tactic for Galois relators*)
-  fun per_simp_prover ctxt thm =
-    let
-      val prems = Thm.cprems_of thm
-      val per_prover_tac = per_prover_tac ctxt
-      fun prove_prem prem = Goal.prove_internal ctxt [] prem (fn _ => HEADGOAL per_prover_tac)
-    in try (map prove_prem) prems |> Option.map (curry (op OF) thm) end
-  fun transport_relator_rewrite ctxt thm =
-    let
-      val transport_defs = Transport_Defs.get ctxt
-      val transport_relator_rewrites = Transport_Relator_Rewrites.get ctxt
-      val ctxt = (clear_simpset ctxt) addsimps transport_relator_rewrites
-    in
-      Local_Defs.fold ctxt transport_defs thm
-      |> Raw_Simplifier.rewrite_thm (false, false, false) per_simp_prover ctxt
-    end
-  fun transport_relator_rewrite_tac ctxt =
-    EqSubst.eqsubst_tac ctxt [0] (Transport_Relator_Rewrites.get ctxt)
-    THEN_ALL_NEW TRY o SOLVED' (per_prover_tac ctxt)
-\<close>
-
-method_setup transport_relator_rewrite =
-  \<open>Scan.succeed (SIMPLE_METHOD' o transport_relator_rewrite_tac)\<close>
-  "Rewrite Transport relator"
-
-
-paragraph \<open>The trp\_term command\<close>
-
-text \<open>Parsing\<close>
-
-ML\<open>
-  @{parse_entries (struct) PA [L, R, x, y]}
-  val parse_cmd_entries =
-    let
-      val parse_value = PA.parse_entry Parse.term Parse.term Parse.term Parse.term
-      val parse_entry = Parse_Key_Value.parse_entry PA.parse_key Parse_Util.eq parse_value
-    in PA.parse_entries_required Parse.and_list1 [PA.key PA.x] parse_entry (PA.empty_entries ()) end
-\<close>
-
-ML\<open>
-  (*some utilities to destruct terms*)
-  val transport_per_start_thm = @{thm "transport.transport_per_start"}
-  val related_if_transport_per_thm = @{thm "transport.left_Galois_if_transport_per"}
-  fun dest_transport_per \<^Const_>\<open>transport.transport_per S T for L R l r x y\<close> =
-    ((S, T), (L, R, l, r, x, y))
-  val dest_transport_per_y = dest_transport_per #> (fn (_, (_, _, _, _, _, y)) => y)
-
-  fun mk_hom_Galois Ta Tb L R r x y =
-    \<^Const>\<open>galois_rel.Galois Ta Ta Tb Tb for L R r x y\<close>
-  fun dest_hom_Galois \<^Const_>\<open>galois_rel.Galois Ta _ Tb _ for L R r x y\<close> =
-    ((Ta, Tb), (L, R, r, x, y))
-  val dest_hom_Galois_y = dest_hom_Galois #> (fn (_, (_, _, _, _, y)) => y)
-
-  (*bindings for generated theorems and definitions*)
-  val binding_transport_per = \<^binding>\<open>transport_per\<close>
-  val binding_per = \<^binding>\<open>per\<close>
-  val binding_in_dom = \<^binding>\<open>in_dom\<close>
-  val binding_related = \<^binding>\<open>related\<close>
-  val binding_related_rewritten = \<^binding>\<open>related'\<close>
-  val binding_def_simplified = \<^binding>\<open>eq\<close>
-  val binding_def_eta_expanded_simplified = \<^binding>\<open>app_eq\<close>
-
-  fun note_facts (binding, mixfix) ctxt related_thm y binding_thms_attribs =
-    let
-      val ((_, (_, y_def)), ctxt) = Util.create_local_theory_def (binding, mixfix) [] y ctxt
-      (*create simplified definition theorems*)
-      val transport_defs = Transport_Defs.get ctxt
-      val (y_def_simplified, y_def_eta_expanded_simplified) =
-        simp_transported_def ctxt transport_defs y_def
-      (*create relatedness theorems*)
-      val related_thm_rewritten = transport_relator_rewrite ctxt related_thm
-      fun prepare_fact (suffix, thm, attribs) =
-        let
-          val binding = (Util.add_suffix binding suffix, [])
-          val ctxt = (clear_simpset ctxt) addsimps transport_defs
-          val folded_thm =
-            (*fold definition of transported term*)
-            Local_Defs.fold ctxt [y_def] thm
-            (*simplify other transport definitions in theorem*)
-            |> (Simplifier.rewrite ctxt |> Conversion_Util.thm_conv)
-          val thm_attribs = ([folded_thm], attribs)
-        in (binding, [thm_attribs]) end
-      val facts = map prepare_fact ([
-          (binding_related, related_thm, []),
-          (binding_related_rewritten, related_thm_rewritten,
-            [Util.attrib_to_src (Binding.pos_of binding) Transport_Related_Intros.add]),
-          (binding_def_simplified, y_def_simplified, []),
-          (binding_def_eta_expanded_simplified, y_def_eta_expanded_simplified, [])
-        ] @ binding_thms_attribs)
-    in Local_Theory.notes facts ctxt |> snd end
-
-  (*black-box transport as described in the Transport paper*)
-  fun after_qed_blackbox (binding, mixfix) [thms as [per_thm, in_dom_thm]] ctxt =
-    let
-      val transport_per_thm = List.foldl (op INCR_COMP) transport_per_start_thm thms
-      (*fix possibly occurring meta type variables*)
-      val ((_, [transport_per_thm]), ctxt) = Variable.importT [transport_per_thm] ctxt
-      val y = Util.real_thm_concl transport_per_thm |> dest_transport_per_y
-
-      val related_thm = transport_per_thm INCR_COMP related_if_transport_per_thm
-      val binding_thms = [
-          (binding_transport_per, transport_per_thm, []),
-          (binding_per, per_thm, []),
-          (binding_in_dom, in_dom_thm,
-            [Util.attrib_to_src (Binding.pos_of binding) Transport_in_dom.add])
-        ]
-    in note_facts (binding, mixfix) ctxt related_thm y binding_thms end
-
-  (*experimental white-box transport support*)
-  fun after_qed_whitebox (binding, mixfix) [[related_thm]] ctxt =
-    let
-      (*fix possibly occurring meta type variables*)
-      val ((_, [related_thm]), ctxt) = Variable.importT [related_thm] ctxt
-      val y = Util.real_thm_concl related_thm |> dest_hom_Galois_y
-    in note_facts (binding, mixfix) ctxt related_thm y [] end
-
-  fun setup_goals_blackbox ctxt (L, R, cx) maxidx =
-    let
-      (*check*)
-      val [cL, cR] = Syntax.check_terms ctxt [L, R] |> map (Thm.cterm_of ctxt)
-      (*instantiate theorem*)
-      val transport_per_start_thm = Thm.incr_indexes (maxidx + 1) transport_per_start_thm
-      val args = [SOME cL, SOME cR, NONE, NONE, SOME cx]
-      val transport_per_start_thm = Drule.infer_instantiate' ctxt args transport_per_start_thm
-      val transport_defs = Transport_Defs.get ctxt
-      val goals = Local_Defs.fold ctxt transport_defs transport_per_start_thm
-        |> Thm.prems_of
-        |> map (rpair [])
-    in goals end
-
-  fun setup_goals_whitebox ctxt (yT, L, R, cx, y) maxidx =
-    let
-      val (r, _) = Term_Util.fresh_var "r" dummyT maxidx
-      (*check*)
-      val Galois = mk_hom_Galois (Thm.typ_of_cterm cx) yT L R r (Thm.term_of cx) y
-        |> Syntax.check_term ctxt
-      val goal = Util.mk_judgement Galois |> rpair []
-    in [goal] end
-
-  fun setup_proof ((((binding, opt_yT, mixfix), params), unfolds), whitebox) lthy =
-    let
-      val ctxt = Util.set_proof_mode_schematic lthy
-      (*type of transported term*)
-      val yT = Option.map (Syntax.read_typ ctxt) opt_yT |> the_default dummyT
-      (*theorems to unfold*)
-      val unfolds = map (Proof_Context.get_fact ctxt o fst) unfolds |> flat
-      (*term to transport*)
-      val cx =
-        (**read term**)
-        Syntax.read_term ctxt (PA.get_x params) |> Thm.cterm_of ctxt
-        (**unfold passed theorems**)
-        |> Drule.cterm_rule (Local_Defs.unfold ctxt unfolds)
-      (*transport relations and transport term goal*)
-      val ([L, R, y], maxidx) =
-        let
-          (**configuration**)
-          val opts = [PA.get_L_safe params, PA.get_R_safe params, PA.get_y_safe params]
-          val opts_default_names = ["L", "R", "y"]
-          val opts_constraints =
-            [Util.mk_hom_rel_type (Thm.typ_of_cterm cx), Util.mk_hom_rel_type yT, yT]
-            |> map Type.constraint
-          (**parse**)
-          val opts = map (Syntax.parse_term ctxt |> Option.map) opts
-          val params_maxidx = Util.list_max (the_default ~1 o Option.map Term.maxidx_of_term)
-            (Thm.maxidx_of_cterm cx) opts
-          fun create_var (NONE, n) maxidx =
-                Term_Util.fresh_var n dummyT params_maxidx ||> Integer.max maxidx
-            | create_var (SOME t, _) created = (t, created)
-          val (ts, maxidx) =
-            fold_map create_var (opts ~~ opts_default_names) params_maxidx
-            |>> map2 I opts_constraints
-        in (ts, maxidx) end
-      (*initialise goals and callback*)
-      val (goals, after_qed) = if whitebox
-        then (setup_goals_whitebox ctxt (yT, L, R, cx, y) maxidx, after_qed_whitebox)
-        (*TODO: consider y in blackbox proofs*)
-        else (setup_goals_blackbox ctxt (L, R, cx) maxidx, after_qed_blackbox)
-    in
-      Proof.theorem NONE (after_qed (binding, mixfix)) [goals] ctxt
-      |> Proof.refine_singleton Util.split_conjunctions
-    end
-
-  val parse_strings =
-    (*binding for transported term*)
-    Parse_Spec.constdecl
-    (*other params*)
-    -- parse_cmd_entries
-    (*optionally pass unfold theorems in case of white-box transports*)
-    -- Scan.optional (Parse.reserved "unfold" |-- Parse.thms1) []
-    (*use a bang "!" to start white-box transport mode (experimental)*)
-    -- Parse.opt_bang
-
-  val _ =
-    Outer_Syntax.local_theory_to_proof \<^command_keyword>\<open>trp_term\<close>
-      "transport of definition" (parse_strings >> setup_proof)
-\<close>
-
-paragraph \<open>Experimental White-Box Prover\<close>
-
-lemmas related_Fun_Rel_combI = Dep_Fun_Rel_relD[where ?S="\<lambda>_ _. S" for S, rotated]
-lemma related_Fun_Rel_lambdaI:
-  assumes "\<And>x y. R x y \<Longrightarrow> S (f x) (g y)"
-  and "T = (R \<Rrightarrow> S)"
-  shows "T f g"
-  using assms by blast
-
-ML\<open>
-  val any_match_resolve_related_tac =
-    let fun unif binders = Higher_Ordern_Pattern_First_Decomp_Unification.e_match
-      Unification_Util.match_types unif Unification_Combinator.fail_unify binders
-    in
-      Unify_Resolve_Base.unify_resolve_any_tac
-        Higher_Ordern_Pattern_First_Decomp_Unification.norms_match unif
-    end
-
-  val related_comb_tac = any_match_resolve_related_tac @{thms related_Fun_Rel_combI}
-  val related_lambda_tac = any_match_resolve_related_tac @{thms related_Fun_Rel_lambdaI}
-  val related_tac = any_unify_trp_hints_resolve_tac
-  val related_assume_tac = assume_tac
-
-  fun mk_transport_related_tac cc_comb cc_lambda ctxt =
-    let
-      val transport_related_intros = Transport_Related_Intros.get ctxt
-      val related_tac = related_tac transport_related_intros ctxt
-      val comb_tac = related_comb_tac ctxt
-      val lambda_tac = related_lambda_tac ctxt
-      val assume_tac = related_assume_tac ctxt
-    in
-      Tactic_Util.CONCAT' [
-        related_tac,
-        cc_comb comb_tac,
-        cc_lambda lambda_tac,
-        assume_tac
-      ]
-    end
-  val transport_related_step_tac =
-    let fun cc_comb tac i = tac i
-      THEN prefer_tac i
-      THEN prefer_tac (i + 1)
-    in mk_transport_related_tac cc_comb I end
-  fun transport_related_tac ctxt =
-    let
-      fun transport_related_tac cc =
-        let
-          fun cc_comb tac = tac THEN_ALL_NEW TRY o cc
-          fun cc_lambda tac = tac THEN' TRY o cc
-        in mk_transport_related_tac cc_comb cc_lambda ctxt end
-      fun fix tac i thm = tac (fix tac) i thm
-    in fix transport_related_tac end
-\<close>
-
-method_setup transport_related_prover =
-  \<open>Scan.succeed (SIMPLE_METHOD' o transport_related_tac)\<close>
-  "Relatedness prover for Transport"
-
-ML\<open>
-  fun instantiate_tac name ct ctxt =
-    PRIMITIVE (Drule.infer_instantiate_types ctxt [((name, Thm.typ_of_cterm ct), ct)])
-    |> CHANGED
-
-  val map_dummyT = Term.map_types (K dummyT)
-
-  fun mk_term_skeleton maxidx t =
-    let
-      val consts = Term.add_consts t []
-      val (vars, _) = fold_map (uncurry Term_Util.fresh_var o apfst Long_Name.base_name) consts maxidx
-      val t' = Term.subst_atomic (map2 (pair o Const) consts vars) t
-    in t' end
-
-  fun instantiate_skeleton_tac ctxt =
-    let fun tac ct =
-      let
-        val (x, y) = Util.cdest_judgement ct |> Thm.dest_binop
-        val default_sort = Proof_Context.default_sort ctxt
-        val skeleton =
-          mk_term_skeleton (Thm.maxidx_of_cterm ct) (Thm.term_of x)
-          |> map_dummyT
-          |> Type.constraint (Thm.typ_of_cterm y)
-          |> Syntax.check_term (Util.set_proof_mode_pattern ctxt)
-          (*add sort constraints for type variables*)
-          |> Term.map_types (Term.map_atyps (map_type_tvar (fn (n, _) => TVar (n, default_sort n))))
-          |> Thm.cterm_of ctxt
-      in instantiate_tac (Thm.term_of y |> dest_Var |> fst) skeleton ctxt end
-    in Tactic_Util.CSUBGOAL_DATA I (K o tac) end
-\<close>
-
-ML\<open>
-  fun transport_whitebox_tac ctxt =
-    instantiate_skeleton_tac ctxt
-    THEN' transport_related_tac ctxt
-    THEN_ALL_NEW (
-      TRY o REPEAT1 o transport_relator_rewrite_tac ctxt
-      THEN' TRY o any_unify_trp_hints_resolve_tac @{thms refl} ctxt
-    )
-\<close>
-
-method_setup transport_whitebox_prover =
-  \<open>Scan.succeed (SIMPLE_METHOD' o transport_whitebox_tac)\<close>
-  "Whitebox prover for Transport"
+  transport_id.left_Galois_eq_left[trp_relator_rewrite]
+  transport_Fun_Rel.left_Galois_eq_Fun_Rel_left_Galois[trp_relator_rewrite]
 
 
 end
