Transport/Examples/Typedef/Transport_Typedef.thy
@@ -16,7 +16,7 @@ typedef pint = "{i :: int. 0 \<le> i}" by auto
 interpretation typedef_pint : type_definition Rep_pint Abs_pint "{i :: int. 0 \<le> i}"
   by (fact type_definition_pint)
 
-lemma [transport_relator_rewrite, trp_uhint]:
+lemma [trp_relator_rewrite, trp_uhint]:
   "(\<^bsub>(=\<^bsub>Collect ((\<le>) (0 :: int))\<^esub>)\<^esub>\<lessapprox>\<^bsub>(=) Rep_pint\<^esub>) \<equiv> typedef_pint.AR"
   using typedef_pint.left_Galois_eq_AR by (intro eq_reflection) simp
 
@@ -26,7 +26,7 @@ interpretation typedef_fset :
   type_definition Rep_fset Abs_fset "{s :: 'a set. finite s}"
   by (fact type_definition_fset)
 
-lemma [transport_relator_rewrite, trp_uhint]:
+lemma [trp_relator_rewrite, trp_uhint]:
   "(\<^bsub>(=\<^bsub>{s :: 'a set. finite s}\<^esub>) :: 'a set \<Rightarrow> _\<^esub>\<lessapprox>\<^bsub>(=) Rep_fset\<^esub>) \<equiv> typedef_fset.AR"
   using typedef_fset.left_Galois_eq_AR by (intro eq_reflection) simp
 
@@ -40,128 +40,85 @@ declare
   typedef_fset.partial_equivalence_rel_equivalence[per_intro]
 
 
-lemma one_parametric [transport_in_dom]: "typedef_pint.L 1 1" by auto
+lemma one_parametric [trp_in_dom]: "typedef_pint.L 1 1" by auto
 
 trp_term pint_one :: "pint" where x = "1 :: int"
-  by transport_prover
+  by trp_prover
 
-lemma add_parametric [transport_in_dom]:
+lemma add_parametric [trp_in_dom]:
   "(typedef_pint.L \<Rrightarrow> typedef_pint.L \<Rrightarrow> typedef_pint.L) (+) (+)"
   by (intro Dep_Fun_Rel_relI) (auto intro!: eq_restrictI elim!: eq_restrictE)
 
 trp_term pint_add :: "pint \<Rightarrow> pint \<Rightarrow> pint"
   where x = "(+) :: int \<Rightarrow> _"
-  by transport_prover
+  by trp_prover
 
-lemma empty_parametric [transport_in_dom]: "typedef_fset.L {} {}"
+lemma empty_parametric [trp_in_dom]: "typedef_fset.L {} {}"
   by auto
 
 trp_term fempty :: "'a fset" where x = "{} :: 'a set"
-  by transport_prover
+  by trp_prover
 
 
-lemma insert_parametric [transport_in_dom]:
+lemma insert_parametric [trp_in_dom]:
   "((=) \<Rrightarrow> typedef_fset.L \<Rrightarrow> typedef_fset.L) insert insert"
   by auto
 
 trp_term finsert :: "'a \<Rightarrow> 'a fset \<Rightarrow> 'a fset" where x = insert
   and L = "((=) \<Rrightarrow> typedef_fset.L \<Rrightarrow> typedef_fset.L)"
   and R = "((=) \<Rrightarrow> typedef_fset.R \<Rrightarrow> typedef_fset.R)"
-  by transport_prover
+  by trp_prover
+
+
+(*experiments with white-box transports*)
 
 context
-  notes refl[transport_related_intro]
+  notes refl[trp_related_intro]
 begin
 
 trp_term insert_add_int_fset_whitebox :: "int fset"
   where x = "insert (1 + (1 :: int)) {}" !
-  by transport_whitebox_prover
+  by trp_whitebox_prover
 
-lemma empty_parametric' [transport_related_intro]: "(rel_set R) {} {}"
+lemma empty_parametric' [trp_related_intro]: "(rel_set R) {} {}"
   by (intro Dep_Fun_Rel_relI rel_setI) (auto dest: rel_setD1 rel_setD2)
 
-lemma insert_parametric' [transport_related_intro]:
+lemma insert_parametric' [trp_related_intro]:
   "(R \<Rrightarrow> rel_set R \<Rrightarrow> rel_set R) insert insert"
   by (intro Dep_Fun_Rel_relI rel_setI) (auto dest: rel_setD1 rel_setD2)
 
-(*proven for all natural functors*)
-lemma Galois_set_hint [trp_uhint]:
-  "L \<equiv> rel_set (L1 :: 'a \<Rightarrow> 'a \<Rightarrow> bool) \<Longrightarrow> R \<equiv> rel_set (R1 :: 'b \<Rightarrow> 'b \<Rightarrow> bool)
+context
+  assumes [trp_uhint]:
+  (*proven for all natural functors*)
+  "L \<equiv> rel_set (L1 :: int \<Rightarrow> int \<Rightarrow> bool) \<Longrightarrow> R \<equiv> rel_set (R1 :: pint \<Rightarrow> pint \<Rightarrow> bool)
   \<Longrightarrow> r \<equiv> image r1 \<Longrightarrow> S \<equiv> (\<^bsub>L1\<^esub>\<lessapprox>\<^bsub>R1 r1\<^esub>) \<Longrightarrow> (\<^bsub>L\<^esub>\<lessapprox>\<^bsub>R r\<^esub>) \<equiv> rel_set S"
-  sorry
+begin
 
 trp_term insert_add_pint_set_whitebox :: "pint set"
   where x = "insert (1 + (1 :: int)) {}" !
-  by transport_whitebox_prover
+  by trp_whitebox_prover
 
 print_statement insert_add_int_fset_whitebox_def insert_add_pint_set_whitebox_def
 
 end
+end
 
-lemma image_parametric [transport_in_dom]:
+lemma image_parametric [trp_in_dom]:
   "(((=) \<Rrightarrow> (=)) \<Rrightarrow> typedef_fset.L \<Rrightarrow> typedef_fset.L) image image"
   by (intro Dep_Fun_Rel_relI) auto
 
 trp_term fimage :: "('a \<Rightarrow> 'b) \<Rightarrow> 'a fset \<Rightarrow> 'b fset" where x = image
-  by transport_prover
+  by trp_prover
 
-(*further experiments*)
-(*experiment with compositions*)
+(*experiments with compositions*)
 
 lemma rel_fun_eq_Fun_Rel_rel: "rel_fun = Fun_Rel_rel"
   by (intro ext iffI Dep_Fun_Rel_relI) (auto elim: rel_funE)
 
-lemma image_parametric' [transport_related_intro]:
+lemma image_parametric' [trp_related_intro]:
   "((R \<Rrightarrow> S) \<Rrightarrow> rel_set R \<Rrightarrow> rel_set S) image image"
   using transfer_raw[simplified rel_fun_eq_Fun_Rel_rel Transfer.Rel_def]
   by simp
-
-context
-  fixes L1 R1 l1 r1 L R l r
-  assumes "(L1 \<equiv>\<^bsub>PER\<^esub> R1) l1 r1"
-  defines "L \<equiv> rel_set L1" and "R \<equiv> rel_set R1"
-  and "l \<equiv> image l1" and "r \<equiv> image r1"
-begin
-
-interpretation transport L R l r .
-
-(*proven for all natural functors*)
-lemma transport_per_set: "((\<le>\<^bsub>L\<^esub>) \<equiv>\<^bsub>PER\<^esub> (\<le>\<^bsub>R\<^esub>)) l r" sorry
-
-end
-
-context
-  fixes L1 R1 l1 r1 L R l r
-  assumes per1: "(L1 \<equiv>\<^bsub>PER\<^esub> R1) l1 r1"
-  and compat:
-    "transport_comp.middle_compatible_codom (rel_set R1) typedef_fset.L"
-begin
-
-trp_term fempty_param :: "'b fset"
-  where x = "{} :: 'a set"
-  and L = "transport_comp.L ?L1 ?R1 (?l1 :: 'a set \<Rightarrow> 'b set) ?r1 typedef_fset.L"
-  and R = "transport_comp.L typedef_fset.R typedef_fset.L ?r2 ?l2 ?R1"
-  apply (rule transport_comp.partial_equivalence_rel_equivalenceI)
-    apply (rule transport_per_set[OF per1])
-    apply per_prover
-    apply (fact compat)
-  apply (rule transport_comp.left_relI[where ?y="{}" and ?y'="{}"])
-    apply (auto intro!: galois_rel.left_GaloisI in_codomI empty_transfer)
-  done
-
-end
-
-definition "set_succ \<equiv> image ((+) (1 :: int))"
-
-lemma set_succ_parametric [transport_in_dom]:
-  "(typedef_fset.L \<Rrightarrow> typedef_fset.L) set_succ set_succ"
-  unfolding set_succ_def by auto
-
-trp_term fset_succ :: "int fset \<Rightarrow> int fset"
-  where x = set_succ
-  and L = "typedef_fset.L \<Rrightarrow> typedef_fset.L"
-  and R = "typedef_fset.R \<Rrightarrow> typedef_fset.R"
-  by transport_prover
 
 lemma Galois_id_hint [trp_uhint]:
   "(L :: 'a \<Rightarrow> 'a \<Rightarrow> bool) \<equiv> R \<Longrightarrow> r \<equiv> id \<Longrightarrow> E \<equiv> L \<Longrightarrow> (\<^bsub>L\<^esub>\<lessapprox>\<^bsub>R r\<^esub>) \<equiv> E"
@@ -170,28 +127,68 @@ lemma Galois_id_hint [trp_uhint]:
 lemma Freq [trp_uhint]: "L \<equiv> (=) \<Rrightarrow> (=) \<Longrightarrow> L \<equiv> (=)"
   by auto
 
+context
+  fixes L1 R1 l1 r1 L R l r
+  assumes per1: "(L1 \<equiv>\<^bsub>PER\<^esub> R1) l1 r1"
+  defines "L \<equiv> rel_set L1" and "R \<equiv> rel_set R1"
+  and "l \<equiv> image l1" and "r \<equiv> image r1"
+begin
+
+interpretation transport L R l r .
+
+context
+  (*proven for all natural functors*)
+  assumes transport_per_set: "((\<le>\<^bsub>L\<^esub>) \<equiv>\<^bsub>PER\<^esub> (\<le>\<^bsub>R\<^esub>)) l r"
+  and compat: "transport_comp.middle_compatible_codom R typedef_fset.L"
+begin
+
+trp_term fempty_param :: "'b fset"
+  where x = "{} :: 'a set"
+  and L = "transport_comp.L ?L1 ?R1 (?l1 :: 'a set \<Rightarrow> 'b set) ?r1 typedef_fset.L"
+  and R = "transport_comp.L typedef_fset.R typedef_fset.L ?r2 ?l2 ?R1"
+  apply (rule transport_comp.partial_equivalence_rel_equivalenceI)
+    apply (rule transport_per_set)
+    apply per_prover
+    apply (fact compat)
+  apply (rule transport_comp.left_relI[where ?y="{}" and ?y'="{}"])
+  apply (unfold L_def R_def l_def r_def)
+  apply (auto intro!: galois_rel.left_GaloisI in_codomI empty_transfer)
+  done
+
+definition "set_succ \<equiv> image ((+) (1 :: int))"
+
+lemma set_succ_parametric [trp_in_dom]:
+  "(typedef_fset.L \<Rrightarrow> typedef_fset.L) set_succ set_succ"
+  unfolding set_succ_def by auto
+
+trp_term fset_succ :: "int fset \<Rightarrow> int fset"
+  where x = set_succ
+  and L = "typedef_fset.L \<Rrightarrow> typedef_fset.L"
+  and R = "typedef_fset.R \<Rrightarrow> typedef_fset.R"
+  by trp_prover
+
 trp_term fset_succ' :: "int fset \<Rightarrow> int fset"
   where x = set_succ
   and L = "typedef_fset.L \<Rrightarrow> typedef_fset.L"
   and R = "typedef_fset.R \<Rrightarrow> typedef_fset.R"
   unfold set_succ_def !
-  using refl[transport_related_intro]
-  apply (tactic \<open>instantiate_skeleton_tac @{context} 1\<close>)
-  apply (tactic \<open>transport_related_step_tac @{context} 1\<close>)
-  thm fimage_related'
-  apply (tactic \<open>transport_related_step_tac @{context} 1\<close>)
-  apply (tactic \<open>transport_related_step_tac @{context} 1\<close>)
-  apply (tactic \<open>transport_related_step_tac @{context} 1\<close>)
-  apply (tactic \<open>transport_related_step_tac @{context} 1\<close>)
-  apply (tactic \<open>transport_related_step_tac @{context} 1\<close>)
+  (*current prototype gets lost in this example*)
+  using refl[trp_related_intro]
+  apply (tactic \<open>Transport.instantiate_skeleton_tac @{context} 1\<close>)
+  apply (tactic \<open>Transport.transport_related_step_tac @{context} 1\<close>)
+  apply (tactic \<open>Transport.transport_related_step_tac @{context} 1\<close>)
+  apply (tactic \<open>Transport.transport_related_step_tac @{context} 1\<close>)
+  apply (tactic \<open>Transport.transport_related_step_tac @{context} 1\<close>)
+  apply (tactic \<open>Transport.transport_related_step_tac @{context} 1\<close>)
+  apply (tactic \<open>Transport.transport_related_step_tac @{context} 1\<close>)
   apply assumption
   apply assumption
   prefer 3
-  apply (tactic \<open>transport_related_step_tac @{context} 1\<close>)
-  apply (tactic \<open>transport_related_step_tac @{context} 1\<close>)
-  apply (fold transport_def)
-  apply (transport_relator_rewrite)+
-  apply (unfold transport_def)
+  apply (tactic \<open>Transport.transport_related_step_tac @{context} 1\<close>)
+  apply (tactic \<open>Transport.transport_related_step_tac @{context} 1\<close>)
+  apply (fold trp_def)
+  apply (trp_relator_rewrite)+
+  apply (unfold trp_def)
   apply (trp_hints_resolve refl)
   done
 
@@ -203,22 +200,11 @@ lemma pint_middle_compat:
 
 trp_term pint_fset_succ :: "pint fset \<Rightarrow> pint fset"
   where x = "set_succ :: int set \<Rightarrow> int set"
-  apply (rule transport_Fun_Rel.partial_equivalence_rel_equivalenceI)
-    apply (rule transport_comp.partial_equivalence_rel_equivalenceI)
-      apply (rule transport_per_set)
-      apply (rule typedef_pint.partial_equivalence_rel_equivalence)
-      apply per_prover
-      apply (fact pint_middle_compat)
-    apply (rule transport_comp.partial_equivalence_rel_equivalenceI)
-      apply (rule transport_per_set)
-      apply (rule typedef_pint.partial_equivalence_rel_equivalence)
-      apply per_prover
-      apply (fact pint_middle_compat)
-  apply (simp add: transport_def)
-  apply (intro Dep_Fun_Rel_relI)
+  (*automation for composition not supported as of now*)
   oops
 
 end
-
+end
+end
 
 end
